code/experimental/pkcs/Spec/Hacl.PKCS11.Types.fst
@@ -1,5 +1,224 @@
 module Hacl.PKCS11.Types
 
+open FStar.UInt32
+open FStar.UInt8
+
+open FStar.Seq
+
 type _HACL_Curve_ID = 
   |Curve25519
   |CurveP256
+
+
+
+(* Zero-level types *)
+type uint8_t = FStar.UInt8.t 
+type uint32_t = a: nat {a < pow2 32}
+
+(* First-level types *)
+
+(* 
+/* an unsigned value, at least 32 bits long */
+typedef unsigned long int CK_ULONG; 
+*)
+
+type _CK_ULONG = uint32_t
+
+
+(*
+/* CK_ATTRIBUTE_TYPE is a value that identifies an attribute
+ * type */
+typedef CK_ULONG          CK_ATTRIBUTE_TYPE;
+*)
+type _CK_ATTRIBUTE_TYPE = 
+  |CKA_CLASS
+  |CKA_PRIVATE
+  |CKA_KEY_TYPE
+  |CKA_SIGN
+  |CKA_VERIFY
+  |CKA_LOCAL
+  |CKA_SECRET_KEY
+  |CKA_TOKEN
+  |CKA_MODIFIABLE
+  |CKA_LABEL
+  |CKA_COPYABLE
+  |CKA_DESTROYABLE
+  |CKA_ID
+  |CKA_START_DATE
+  |CKA_END_DATE
+  |CKA_DERIVED
+  |CKA_KEY_GEN_MECHANISM
+  |CKA_ALLOWED_MECHANISMS
+  |CKA_SUBJECT
+  |CKA_ENCRYPT
+  |CKA_VERIFY_RECOVER
+  |CKA_WRAP
+  |CKA_TRUSTED
+  |CKA_WRAP_TEMPLATE
+  |CKA_PUBLIC_KEY_INFO
+  |CKA_SENSITIVE
+  |CKA_DECRYPT
+  |CKA_SIGN_RECOVER
+  |CKA_UNWRAP
+  |CKA_EXTRACTABLE
+  |CKA_ALWAYS_SENSITIVE
+  |CKA_NEVER_EXTRACTABLE
+  |CKA_WRAP_WITH_TRUSTED
+  |CKA_UNWRAP_TEMPLATE
+  |CKA_ALWAYS_AUTHENTICATE
+  |CKA_CHECK_VALUE
+  |CKA_EC_PARAMS 
+  |CKA_VALUE
+
+
+(*
+/* CK_OBJECT_CLASS is a value that identifies the classes (or
+ * types) of objects that Cryptoki recognizes.  It is defined
+ * as follows: */
+typedef CK_ULONG          CK_OBJECT_CLASS;
+*)
+
+(* /* The following classes of objects are defined: */
+#define CKO_DATA              0x00000000UL
+#define CKO_CERTIFICATE       0x00000001UL
+#define CKO_PUBLIC_KEY        0x00000002UL
+#define CKO_PRIVATE_KEY       0x00000003UL
+#define CKO_SECRET_KEY        0x00000004UL
+#define CKO_HW_FEATURE        0x00000005UL
+#define CKO_DOMAIN_PARAMETERS 0x00000006UL
+#define CKO_MECHANISM         0x00000007UL
+#define CKO_OTP_KEY           0x00000008UL
+
+#define CKO_VENDOR_DEFINED    0x80000000UL
+*)
+
+type _CK_OBJECT_CLASS = 
+  |CKO_DATA
+  |CKO_CERTIFICATE
+  |CKO_PUBLIC_KEY
+  |CKO_PRIVATE_KEY
+  |CKO_SECRET_KEY
+  |CKO_HW_FEATURE
+  |CKO_DOMAIN_PARAMETERS
+  |CKO_MECHANISM
+  |CKO_OTP_KEY
+  |CKO_VENDOR_DEFINED
+
+
+type _CK_OBJECT_CLASS_EXTENDED = 
+  |CKO_OBJECT
+  |CKO_STORAGE
+  |CKO_KEY
+
+
+let getAttributesForTypeExtended: t: _CK_OBJECT_CLASS_EXTENDED -> seq _CK_ATTRIBUTE_TYPE = function
+  |CKO_OBJECT -> seq_of_list [CKA_CLASS]
+  |CKO_KEY -> seq_of_list [CKA_TOKEN; CKA_PRIVATE; CKA_MODIFIABLE; CKA_LABEL; CKA_COPYABLE; CKA_DESTROYABLE]
+  |CKO_STORAGE -> seq_of_list [CKA_KEY_TYPE; CKA_ID; CKA_END_DATE; CKA_DERIVED; CKA_LOCAL; CKA_KEY_GEN_MECHANISM; CKA_ALLOWED_MECHANISMS]
+
+let getAttributesForType: t: _CK_OBJECT_CLASS -> seq _CK_ATTRIBUTE_TYPE = function 
+  |CKO_SECRET_KEY -> (seq_of_list 
+    [CKA_CLASS; CKA_TOKEN; CKA_PRIVATE; CKA_MODIFIABLE; CKA_LABEL; CKA_COPYABLE; CKA_DESTROYABLE;
+    CKA_KEY_TYPE; CKA_ID; CKA_END_DATE; CKA_DERIVED; CKA_LOCAL; CKA_KEY_GEN_MECHANISM; CKA_ALLOWED_MECHANISMS; CKA_SENSITIVE; CKA_ENCRYPT; CKA_DECRYPT; CKA_SIGN; CKA_VERIFY; 
+    CKA_WRAP; CKA_UNWRAP; CKA_EXTRACTABLE; CKA_ALWAYS_SENSITIVE; CKA_NEVER_EXTRACTABLE])
+  |_ -> Seq.empty
+
+
+(* /* CK_KEY_TYPE is a value that identifies a key type */
+typedef CK_ULONG          CK_KEY_TYPE;
+*)
+type _CK_KEY_TYPE = 
+  |CKK_RSA
+  |CKK_DSA
+  |CKK_DH
+  |CKK_EC 
+  (*and much more *)
+
+
+(*
+/* CK_MECHANISM_TYPE is a value that identifies a mechanism
+ * type */
+typedef CK_ULONG          CK_MECHANISM_TYPE;*)
+type _CK_MECHANISM_TYPE = 
+  |CKM_RSA_PKCS_KEY_PAIR_GEN
+  |CKM_DSA
+  |CKM_EC_KEY_PAIR_GEN
+  |CKM_ECDSA
+  |CKM_AES_KEY_GEN
+  (* and traditionally much more *)
+
+
+let _ck_attribute_get_type: _CK_ATTRIBUTE_TYPE -> Tot Type0 = function
+  |CKA_CLASS -> _CK_OBJECT_CLASS
+  |CKA_SIGN -> bool
+  |CKA_VERIFY -> bool
+  |CKA_LOCAL -> bool
+  |CKA_TOKEN -> bool
+  |CKA_PRIVATE -> bool
+  |CKA_MODIFIABLE -> bool
+  |CKA_LABEL -> uint32_t
+  |CKA_COPYABLE -> bool
+  |CKA_DESTROYABLE -> bool
+  |CKA_KEY_TYPE -> _CK_KEY_TYPE
+  |CKA_ID -> uint32_t
+  |CKA_START_DATE -> uint32_t
+  |CKA_END_DATE -> uint32_t
+  |CKA_DERIVED -> bool
+  |CKA_LOCAL -> bool
+  |CKA_KEY_GEN_MECHANISM -> _CK_MECHANISM_TYPE
+  |CKA_ALLOWED_MECHANISMS -> _CK_MECHANISM_TYPE
+  |CKA_SUBJECT -> uint32_t 
+  |CKA_ENCRYPT -> bool 
+  |CKA_DECRYPT -> bool
+  |CKA_VERIFY -> bool
+  |CKA_VERIFY_RECOVER -> bool
+  |CKA_WRAP -> bool
+  |CKA_TRUSTED -> bool
+  |CKA_WRAP_TEMPLATE -> _CK_ATTRIBUTE_TYPE
+  |CKA_PUBLIC_KEY_INFO -> uint32_t
+  |CKA_SENSITIVE -> bool
+  |CKA_DECRYPT -> bool
+  |CKA_SIGN -> bool
+  |CKA_SIGN_RECOVER -> bool
+  |_ -> _CK_ULONG
+  |CKA_EC_PARAMS -> _CK_ULONG
+  |CKA_VALUE -> uint8_t 
+
+
+(* I am not sure that the length is stated for all possible types *)
+let _ck_attribute_get_len: _CK_ATTRIBUTE_TYPE -> Tot (a: option nat {Some? a ==> (match a with Some a -> a) < pow2 32}) = function
+  |CKA_CLASS -> Some 1
+  |CKA_SIGN -> Some 1
+  |CKA_VERIFY -> Some 1
+  |CKA_LOCAL -> Some 1
+  |CKA_TOKEN -> Some 1
+  |CKA_PRIVATE -> Some 1 
+  |CKA_MODIFIABLE -> Some 1
+  |CKA_COPYABLE -> Some 1
+  |CKA_LABEL -> None
+  |CKA_DESTROYABLE -> Some 1
+  |CKA_KEY_TYPE -> Some 1 
+  |CKA_ID -> None
+  |CKA_START_DATE -> Some 3
+  |CKA_END_DATE -> Some 3
+  |CKA_DERIVED -> Some 1
+  |CKA_LOCAL -> Some 1
+  |CKA_KEY_GEN_MECHANISM -> Some 1
+  |CKA_ALLOWED_MECHANISMS -> None
+  |_ -> None
+
+(*/* CK_ATTRIBUTE is a structure that includes the type, length
+ * and value of an attribute */
+*)
+
+type _CK_ATTRIBUTE  = 
+  |A: 
+    aType: _CK_ATTRIBUTE_TYPE -> pValue: seq (_ck_attribute_get_type aType) 
+    {
+      let len = _ck_attribute_get_len aType in 
+      if Some? len then 
+	length pValue = (match len with Some a -> a)
+      else 
+	True
+    } 
+    -> _CK_ATTRIBUTE
