code/experimental/pkcs/Spec/Hacl.PKCS11.Attributes.API.fst
@@ -1,0 +1,22 @@
+module Hacl.PKCS11.Attributes.API
+
+open FStar.Seq
+open Hacl.PKCS11.Types
+open Hacl.PKCS11.Lib
+open Hacl.PKCS11.Lemmas
+
+val _attributesAllPresent: toSearchSequence: seq _CK_ATTRIBUTE -> toFinds: seq _CK_ATTRIBUTE_TYPE -> Tot (r: bool
+  {
+    r == true ==> 
+      (forall (i: nat {i < Seq.length toFinds}). 
+  contains (fun x -> x.aType = (index toFinds i)) toSearchSequence)
+  }
+)
+
+let _attributesAllPresent toSearchSequence toFinds = 
+  let __attributesAllPresent y toFind : r: bool 
+  {r == true <==> contains (fun x -> x.aType = toFind) y} = 
+    match find_l (fun x -> x.aType = toFind) y with 
+    |None -> find_l_none_no_index y (fun x -> x.aType = toFind); false
+    |Some _ -> lemmaFindLExistIfSome (fun x -> x.aType = toFind) y; true in   
+  for_all (__attributesAllPresent toSearchSequence) toFinds 
