code/experimental/pkcs/Spec/Hacl.PKCS11.Lemmas.ObjectTree.fst
@@ -1,0 +1,9 @@
+module Hacl.PKCS11.Lemmas.ObjectTree
+
+open Hacl.PKCS11.Types
+
+(*
+val lemmaSecretKeyIsObject: unit -> Lemma 
+  (
+    let attributesForSKO = getAttributesForType CKO_SECRET_KEY in 
+    _attributesAllPresent 
